A lot of changes: - split the project into more files. I don't know if this makes things   better or worse, due to Coq's insane way of handling namespaces and   imports this will probably be very hard to maintain and extend. If any   on you have a better idea, feel free to change it. - replaced the TPSubst function with the TPSubstitutesInto predicate - introduced predicates TPIsFreeIn and TPIsNotFreeIn - implemented proper alpha conversion for smallsteps (via axiomatic   rename function) - replaced implementation of typing environments as lists with abstract   environments that satisfy some reasonable axioms - proved various lemmas concerning the interplay between typing,   substitution, smallsteps and environment manipulation - proved the preservation theorem - started on the progress theorem
The definition of smallsteps, substitution and free variables should be
okay now (I was able to prove preservation after all ;-) ). Nevertheless
there are still MANY things to work on (i.e. a lot of 'admit's).

I'll try to whip up some documentation in the next days. I finished the
proof of preservation just last night and didn't want to wait any
longer, so the code is still in a state of disarray I'm afraid.

TPSmallSteps.v
@@ -1,11 +1,12 @@
 Module TPSmallSteps.
 
+Require Import Arith.
 Require Import String.
+
+Load TPSemanticSubstitution.
+Export TPSemanticSubstitution.
+
 Open Scope string_scope.
-
-Load TPSyntax.
-Export TPSyntax.
-
 Open Scope Z_scope.
 
 Definition TPEvalOp op n1 n2 :=
@@ -24,167 +25,193 @@ Definition TPEvalOp op n1 n2 :=
     | _, _, _ => TPHang
   end.
 
-Fixpoint TPFreeVars exp :=
-  match exp with
-    | TPExpConst _ => nil
-    | TPExpId id => id :: nil
-    | TPExpApp exp1 exp2 => app (TPFreeVars exp1) (TPFreeVars exp2)
-    | TPExpIf exp1 exp2 exp3 => app (TPFreeVars exp1) (app (TPFreeVars exp2) (TPFreeVars exp3))
-    | TPExpAbstr id exp => filter (ident_eq id) (TPFreeVars exp)
-    | TPExpLet id e1 e2 => app (filter (ident_eq id) (TPFreeVars e2)) (TPFreeVars e1)
-    | TPExpRec id exp => filter (ident_eq id) (TPFreeVars exp)
-  end.
-
-(*
-Fixpoint subst free_ids e e' id :=
-  match e with
-    | TPConstant c => c
-    | TPExpId id' => if string_eq id' id then e' else id'
-    | TPExpAbstr id' e => if string_eq id' id then e else
-      let id'' := new_id free_ids id' in TPExpAbstr id'' (subst (id'' :: free_ids) (subst free_ids e' (TPExpId id'') id) e' id)
-    | _ => TPConstant TPunit
-  end.
-*)
-
-Definition new_id highest_id id := (TPId (id, S highest_id), S highest_id).
-
-(* Substitute id in e by e' *)
-Fixpoint TPSubst (highest_id : nat) e e' id : TPExp * nat :=
-  match e with
-    | TPExpConst c => (e, highest_id)
-    | TPExpId id' =>
-      if ident_eq id' id
-        then (e', highest_id)
-        else (TPExpId id', highest_id)
-    | TPExpIf e1 e2 e3 =>
-      let (e1', n1) := TPSubst highest_id e1 e' id in
-        let (e2', n2) := TPSubst n1 e2 e' id in
-          let (e3', n3) := TPSubst n2 e3 e' id in
-            (TPIf e1' e2' e3', n3)
-    | TPExpApp e1 e2 =>
-      let (e1', n1) := TPSubst highest_id e1 e' id in
-        let (e2', n2) := TPSubst n1 e2 e' id in
-         (TPExpApp e1' e2', n2)
-    | TPExpAbstr id' e =>
-      if ident_eq id' id
-        then (e, highest_id)
-        else let (e1, n) := TPSubst highest_id e e' id in (TPExpAbstr id' e1, n)
-    | TPExpLet id' e1 e2 =>
-      let (e1', n1) := TPSubst highest_id e1 e' id in
-        let (e2', n2) := TPSubst n1 e2 e' id in
-          (TPExpLet id' e1' (if ident_eq id' id then e2 else e2'), n2)
-    | TPExpRec id' e =>
-      if ident_eq id' id
-        then (e, highest_id)
-        else let (e'', n) := TPSubst highest_id e e' id in (TPExpRec id' e'', n)
-  end.
-
 (* TODO Figure out, whether this definition is correct. *)
-Inductive TPMakesSmallstep: nat -> TPExp -> TPExp * nat -> Prop :=
-| smallstep_op: forall idx n1 n2 op,
-  TPMakesSmallstep idx (TPApp (TPApp (TPOp op) (TPInt n1)) (TPInt n2)) (TPEvalOp op (TPInt n1) (TPInt n2), idx)
-| smallstep_betav: forall idx id exp v,
-  TPIsValue v -> TPMakesSmallstep idx (TPApp (TPAbstr id exp) v) (TPSubst idx exp v id)
-| smallstep_appleft: forall idx idx' exp1 exp1' exp2,
-  TPMakesSmallstep idx exp1 (exp1', idx') -> TPMakesSmallstep idx (TPApp exp1 exp2) (TPApp exp1' exp2, idx')
-| smallstep_appright: forall idx idx' exp exp' v,
-  TPIsValue v -> TPMakesSmallstep idx exp (exp', idx') -> TPMakesSmallstep idx' (TPApp v exp) (TPApp v exp', idx')
-| smallstep_condeval: forall idx idx' exp0 exp0' exp1 exp2,
-  TPMakesSmallstep idx exp0 (exp0', idx') -> TPMakesSmallstep idx' (TPIf exp0 exp1 exp2) (TPIf exp0' exp1 exp2, idx')
-| smallstep_condtrue: forall idx exp1 exp2,
-  TPMakesSmallstep idx (TPIf TPTrue exp1 exp2) (exp1, idx)
-| smallstep_condfalse: forall idx exp1 exp2,
-  TPMakesSmallstep idx (TPIf TPFalse exp1 exp2) (exp2, idx)
-| smallstep_leteval: forall idx idx' id exp1 exp1' exp2,
-  TPMakesSmallstep idx exp1 (exp1', idx') -> TPMakesSmallstep idx' (TPLet id exp1 exp2) (TPLet id exp1' exp2, idx')
-| smallstep_letexec: forall idx id exp v,
-  TPIsValue v -> TPMakesSmallstep idx (TPLet id v exp) (TPSubst idx exp v id).
+Inductive TPMakesSmallstep: TPExp -> TPExp -> Prop :=
+| smallstep_op: forall n1 n2 op,
+  TPMakesSmallstep (TPApp (TPApp (TPOp op) (TPInt n1)) (TPInt n2)) (TPEvalOp op (TPInt n1) (TPInt n2))
+| smallstep_betav: forall id exp exp' v,
+  TPIsValue v -> TPSubstitutesInto exp id v exp' -> TPMakesSmallstep (TPApp (TPAbstr id exp) v) exp'
+| smallstep_appleft: forall exp1 exp1' exp2,
+  TPMakesSmallstep exp1 exp1' -> TPMakesSmallstep (TPApp exp1 exp2) (TPApp exp1' exp2)
+| smallstep_appright: forall exp exp' v,
+  TPIsValue v -> TPMakesSmallstep exp exp' -> TPMakesSmallstep (TPApp v exp) (TPApp v exp')
+| smallstep_condeval: forall exp0 exp0' exp1 exp2,
+  TPMakesSmallstep exp0 exp0' -> TPMakesSmallstep (TPIf exp0 exp1 exp2) (TPIf exp0' exp1 exp2)
+| smallstep_condtrue: forall exp1 exp2,
+  TPMakesSmallstep (TPIf TPTrue exp1 exp2) exp1
+| smallstep_condfalse: forall exp1 exp2,
+  TPMakesSmallstep (TPIf TPFalse exp1 exp2) exp2
+| smallstep_leteval: forall id exp1 exp1' exp2,
+  TPMakesSmallstep exp1 exp1' -> TPMakesSmallstep (TPLet id exp1 exp2) (TPLet id exp1' exp2)
+| smallstep_letexec: forall id exp exp' v,
+  TPIsValue v -> TPSubstitutesInto exp id v exp' -> TPMakesSmallstep (TPLet id v exp) exp'
+| smallstep_unfold: forall id exp exp',
+  TPSubstitutesInto exp id (TPRec id exp) exp' -> TPMakesSmallstep (TPRec id exp) exp'.
 
-Inductive NonEmptyList (A: Type) :=
-| Singleton: A -> NonEmptyList A
-| Cons: A -> NonEmptyList A -> NonEmptyList A.
-
-Implicit Arguments Singleton [A].
-Implicit Arguments Cons [A].
-
-Definition first {A: Type}(l: NonEmptyList A) := match l with
-| Singleton a => a
-| Cons a l' => a
-end.
-
-Fixpoint last {A: Type}(l: NonEmptyList A) := match l with
-| Singleton a => a
-| Cons a l' => (last l')
-end.
-
-Fixpoint length {A: Type}(l: NonEmptyList A) := match l with
-| Singleton a => 1%nat
-| Cons a l' => S (length l')
-end.
-
-Fixpoint nth_default {A: Type}(def: A)(n: nat)(l: NonEmptyList A) := match n,l with
-| O, l => first l
-| S n', Cons a l' => nth_default def n' l'
-| S n', Singleton a => def
-end.
-
-Definition TPMultipleSmallsteps exp exp':= 
-exists steps: NonEmptyList TPExp,
-first steps = exp ->
-last steps = exp' ->
-forall idx n, (n < ((length steps)-1))%nat -> TPMakesSmallstep idx (nth_default TPExn n steps) (nth_default TPExn (n+1) steps, idx).
-
-Definition step0 := (TPLet ("square", 0%nat) (TPAbstr ("x", 1%nat) (TPApp (TPApp TPMult (TPId ("x", 1%nat))) (TPId ("x",1%nat)))) (TPApp (TPId ("square", 0%nat))(TPApp (TPId ("square", 0%nat)) (TPInt 5)))).
-Definition step1 := (TPApp (TPAbstr ("x", 1%nat) (TPApp (TPApp TPMult (TPId ("x", 1%nat))) (TPId ("x", 1%nat))))(TPApp (TPAbstr ("x", 1%nat) (TPApp (TPApp TPMult (TPId ("x", 1%nat))) (TPId ("x", 1%nat)))) (TPInt 5))).
-Definition step2 := (TPApp (TPAbstr ("x", 1%nat) (TPApp (TPApp TPMult (TPId ("x", 1%nat))) (TPId ("x", 1%nat))))(TPApp (TPApp TPMult (TPInt 5)) (TPInt 5))).
-Definition step3 := (TPApp (TPAbstr ("x", 1%nat) (TPApp (TPApp TPMult (TPId ("x", 1%nat))) (TPId ("x", 1%nat))))(TPInt 25)).
-Definition step4 := (TPApp (TPApp TPMult (TPInt 25)) (TPInt 25)).
-Definition step5 := TPInt 625.
-
-Lemma less_nat_cases: forall k n: nat, (k < (S n) <-> k < n \/ k = n)%nat.
+Lemma values_dont_progress: forall v, TPIsValue v -> forall exp, ~ TPMakesSmallstep v exp.
 Proof.
-  intros k n.
-  split; intros H.
-  (* => *)
-    apply lt_n_Sm_le in H.
-    case_eq (beq_nat k n); intros Heq.
-      (* Case: true *)
-      right. apply beq_nat_true_iff in Heq. exact Heq.
-      (* Case: false *)
-      left. apply beq_nat_false_iff in Heq.
-      apply nat_total_order in Heq. destruct Heq as [Heq | Heq].
-        (* Case: k < n *)
-        exact Heq.
-        (* Case: k > n *)
-        apply le_lt_trans with (n:=k) in Heq.
-          contradict Heq. apply lt_irrefl.
-          exact H. 
-  (* <= *)
-    destruct H as [H | H].
-      apply lt_S. exact H.
-      rewrite H. constructor.
+  intros v H exp Hsmallstep.
+  induction Hsmallstep; try (now inversion H).
+    inversion H. apply IHHsmallstep. rewrite <- H0. constructor.
 Qed.
 
-Example test1: TPMultipleSmallsteps step0 step5.
+Lemma smallsteps_are_deterministic: forall exp exp1 exp2, TPMakesSmallstep exp exp1 -> TPMakesSmallstep exp exp2 -> exp1 = exp2.
 Proof.
-  unfold TPMultipleSmallsteps.
-  exists (Cons step0 (Cons step1 (Cons step2 (Cons step3 (Cons step4 (Singleton step5)))))).
-  intros Hfirst Hlast n idx Hn.
-  clear Hfirst. clear Hlast. simpl in Hn.
-  
-  repeat ((try (apply lt_n_Sm_le in Hn; apply le_n_0_eq in Hn; symmetry in Hn)) || (try (apply less_nat_cases in Hn; destruct Hn as [Hn | H])));
-  try rename H into Hn; rewrite Hn; simpl; repeat constructor.
-  apply smallstep_appright with (idx := n).
-  now apply TPAbstrIsValue.
-  assert (H : TPSubst n (TPApp (TPApp TPMult (TPId ("x", 1%nat))) (TPId ("x", 1%nat))) (TPInt 5) ("x", 1%nat) = (TPApp (TPApp TPMult (TPInt 5)) (TPInt 5), n)).
-  simpl; unfold TPApp; unfold TPMult; now reflexivity.
-  rewrite <- H.
-  apply smallstep_betav.
-  now apply TPConstIsValue.
-  apply smallstep_appright with (idx := n).
-  now apply TPAbstrIsValue.
-  apply smallstep_op.
+  intros exp exp1 exp2 Hexp1.
+  generalize dependent exp2.
+    induction Hexp1; intros exp2' Hexp2.
+      (**)
+      inversion Hexp2.
+        reflexivity.
+        inversion H2.
+          contradict H6. apply values_dont_progress. constructor.
+          contradict H7. apply values_dont_progress. constructor.
+        contradict H3. apply values_dont_progress. constructor.
+      (**)
+      inversion Hexp2.
+        apply substitution_is_deterministic with (exp:=exp)(id:=id)(v:=v).
+          assumption.
+          assumption.
+        contradict H4. apply values_dont_progress. constructor.
+        contradict H5. apply values_dont_progress. assumption.
+      (**)
+      inversion Hexp2.
+        contradict Hexp1. apply values_dont_progress. rewrite <- H0. constructor. constructor.
+        contradict Hexp1. apply values_dont_progress. rewrite <- H. constructor.
+        rewrite IHHexp1 with (exp2:=exp1'0).
+          reflexivity.
+          assumption.
+        contradict Hexp1. apply values_dont_progress. assumption.
+      (**)
+      inversion Hexp2.
+        contradict Hexp1. apply values_dont_progress. rewrite <- H2. constructor.
+        contradict Hexp1. apply values_dont_progress. assumption.
+        contradict H3. apply values_dont_progress. assumption.
+        rewrite IHHexp1 with (exp2:=exp'0).
+          reflexivity.
+          assumption.
+      (**)
+      inversion Hexp2.
+        admit.
+        contradict Hexp1. apply values_dont_progress. rewrite <- H0. constructor.
+        contradict Hexp1. apply values_dont_progress. rewrite <- H0. constructor.
+      (**)
+      inversion Hexp2.
+        contradict H3. apply values_dont_progress. constructor.
+        reflexivity.
+      (**)
+      inversion Hexp2.
+        contradict H3. apply values_dont_progress. constructor.
+        reflexivity.
+      (**)
+      inversion Hexp2.
+        rewrite IHHexp1 with (exp2:=exp1'0).
+          reflexivity.
+          assumption.
+        contradict Hexp1. apply values_dont_progress. assumption. 
+      (**)
+      inversion_clear Hexp2.
+        contradict H1. apply values_dont_progress. assumption.
+        apply substitution_is_deterministic with (exp:=exp)(id:=id)(v:=v).
+          assumption.
+          assumption.
+      (**)
+      inversion Hexp2. apply substitution_is_deterministic with (exp:=exp)(id:=id)(v:=(TPRec id exp)).
+        assumption.
+        assumption.
 Qed.
+
+Lemma smallsteps_dont_free_ids: forall id exp exp', TPMakesSmallstep exp exp' -> TPIsNotFreeIn id exp -> TPIsNotFreeIn id exp'.
+Proof.
+  intros id exp exp' Hsmallstep Hnotfree.
+  induction Hsmallstep.
+    (**)
+    destruct op; simpl; constructor.
+    (**)
+    inversion_clear Hnotfree. destruct H1 as [H1 H1'].
+    inversion H1.
+      apply unfree_id_in_subst_exp with (exp:=exp)(sexp:=v).
+        rewrite <- H4. assumption.
+        assumption.
+      clear H3 exp0 H2 id' H4 id1. apply subst_doesnt_free_different_ids with (exp:=exp)(sexp:=v)(id:=id0).
+        apply not_eq_sym. assumption.
+        assumption.
+        assumption.
+    (**)
+    constructor. inversion_clear Hnotfree. destruct H as [H0 H1].
+    split.
+      apply IHHsmallstep. assumption.
+      assumption.
+    (**)
+    constructor. inversion_clear Hnotfree. destruct H0 as [H0 H1].
+    split.
+      assumption.
+      apply IHHsmallstep. assumption.
+    (**)
+    constructor. inversion_clear Hnotfree. destruct H as [H0 [H1 H2]].
+    split; try split.
+      apply IHHsmallstep. assumption.
+      assumption.
+      assumption.
+    (**)
+    inversion_clear Hnotfree. destruct H as [H0 [H1 H2]]. assumption.
+    (**)
+    inversion_clear Hnotfree. destruct H as [H0 [H1 H2]]. assumption.
+    (**)
+    inversion_clear Hnotfree. destruct H.
+      constructor.
+        left. assumption.
+        apply IHHsmallstep. assumption.
+      constructor.
+        right. assumption.
+        apply IHHsmallstep. assumption.
+    (**)
+    inversion_clear Hnotfree. destruct H1 as [[H1 H1'] | H1].
+      apply subst_doesnt_free_different_ids with (exp:=exp)(sexp:=v)(id:=id0).
+        apply not_eq_sym. assumption.
+        assumption.
+        assumption.
+      apply unfree_id_in_subst_exp with (exp:=exp)(sexp:=v).
+        assumption.
+        rewrite H1. assumption.
+    (**)
+    inversion Hnotfree.
+      apply unfree_id_in_subst_exp with (exp:=exp)(sexp:=(TPRec id0 exp)).
+        constructor.
+        assumption.
+      apply subst_doesnt_free_different_ids with (exp:=exp)(sexp:=(TPRec id0 exp))(id:=id0).
+        apply not_eq_sym. assumption.
+        assumption.
+        assumption.
+Qed.
+
+Lemma smallsteps_dont_unfree_ids: forall id exp exp', TPMakesSmallstep exp exp' -> TPIsFreeIn id exp -> TPIsFreeIn id exp'.
+Proof.
+  intros id exp exp' Hsmallstep Hfree.
+  generalize dependent id.
+  induction Hsmallstep; intros id' Hfree.
+    (**)
+    contradict Hfree. apply TPIsNotFreeIn_consist. constructor. split.
+      constructor. split; constructor.
+      constructor.
+    (**)
+    inversion_clear Hfree. destruct H1.
+      inversion_clear H1. apply subst_doesnt_unfree_different_ids with (exp:=exp)(sexp:=v)(id:=id).
+        apply not_eq_sym. assumption.
+        assumption.
+        assumption.
+      apply free_id_in_subst_exp with (exp:=exp)(sexp:=v).
+        assumption.
+        admit.
+    (**)
+    (**)
+    (**)
+    (**)
+    (**)
+    (**)
+    (**)
+    (**)
+Admitted.
 
 End TPSmallSteps.
 
