TPTyping.v
@@ -1,7 +1,7 @@
 Module TPTyping.
 
 Load TPSmallSteps.
-Export TPSmallSteps.
+Import TPSmallSteps.
 
 Require Import List.
 Require Import String.
@@ -15,7 +15,6 @@ Inductive TPType :=
 | TPTypeError.
 
 (* Shorthands *)
-
 Definition TPTypeIntToInt := TPTypeFun TPTypeInt TPTypeInt.
 Definition TPTypeIntToBool := TPTypeFun TPTypeInt TPTypeBool.
 Definition TPTypeIntToIntToInt := TPTypeFun TPTypeInt TPTypeIntToInt.
@@ -50,37 +49,24 @@ Proof.
     rewrite H. clear H. clear t1.
     induction t2; simpl; try reflexivity.
     (* Case: TPTypeFun *)
-    rewrite IHt2_1. rewrite IHt2_2. simpl. now reflexivity.
+    rewrite IHt2_1. rewrite IHt2_2. now tauto.
     (* Case: TPTypeVar *)
     apply string_eq_reflex.
 Qed.
 
-Definition TPTypeEnv := list ((string * nat) * TPType).
+Axiom TPTypeEnv: Set.
+Axiom TPChangeEnv: TPTypeEnv -> TPIdentifier -> TPType -> TPTypeEnv.
+Axiom TPChangeEnv_prop1: forall env env' id tau tau', TPChangeEnv env id tau = TPChangeEnv env' id tau' -> tau = tau'.
 
-Fixpoint change_env id tau env: TPTypeEnv := match env with
-| nil => (id, tau)::nil
-| (id', tau')::env' => if ident_eq id id' then (id, tau)::env' else (id', tau')::(change_env id tau env')
-end.
+Inductive TPIdHasTypeInEnv: TPIdentifier -> TPTypeEnv -> TPType -> Prop :=
+| typeenv_eq: forall env id id' tau, id = id' -> TPIdHasTypeInEnv id (TPChangeEnv env id' tau) tau
+| typeenv_neq: forall env id id' tau tau', id <> id' -> TPIdHasTypeInEnv id env tau -> TPIdHasTypeInEnv id (TPChangeEnv env id' tau') tau.
 
-Lemma change_env_consist: forall env id tau, In (id, tau) (change_env id tau env).
-Proof.
-  intros env id tau.
-  induction env; simpl.
-    left. reflexivity.
-    destruct a as (id', tau'). case_eq (ident_eq id id'); intros H; simpl.
-      left. reflexivity.
-      right. exact IHenv.
-Qed.
-
-Lemma change_env_small: forall env id tau, change_env id tau env = (id, tau) :: nil -> env = nil \/ (exists tau'', env = (id, tau'') :: nil).
-Proof.
-  intros env id tau H.
-  induction env.
-    left. reflexivity.
-    right. destruct a as (id', tau'). case_eq (ident_eq id id'); intros H'; simpl in H; rewrite H' in H; inversion H;
-      exists tau'. apply ident_eq_consist in H'. rewrite H'. reflexivity.
-      symmetry in H1. apply ident_eq_consist in H1. rewrite H1 in H'. contradict H'. discriminate.
-Qed.
+Axiom TypeOfIdUnique: forall id env tau tau', TPIdHasTypeInEnv id env tau -> TPIdHasTypeInEnv id env tau' -> tau = tau'.
+Axiom TypeOfChangedEnvEq: forall id env tau tau', TPIdHasTypeInEnv id (TPChangeEnv env id tau) tau' -> tau = tau'.
+Axiom TypeOfChangedEnvNeq: forall id id' env tau tau', id <> id' -> TPIdHasTypeInEnv id' (TPChangeEnv env id tau) tau' -> TPIdHasTypeInEnv id' env tau'.
+Axiom TypeOfDoubleChangeEnv: forall id env tau tau', TPChangeEnv (TPChangeEnv env id tau) id tau' = TPChangeEnv env id tau'.
+Axiom DoubleChangeSwitch: forall id id' env tau tau', id <> id' -> TPChangeEnv (TPChangeEnv env id tau) id' tau' = TPChangeEnv (TPChangeEnv env id' tau') id tau.
 
 Definition TPTypeOfOp op :=
   match op with
@@ -103,58 +89,475 @@ end.
 
 Inductive TPHasType: TPTypeEnv -> TPExp -> TPType -> Prop :=
 | typerule_const: forall env c tau,
-                      tau = (TPTypeOfConst c) ->
-                        TPHasType env (TPConst c) tau
+                  tau = (TPTypeOfConst c) ->
+                  TPHasType env (TPConst c) tau
 | typerule_id: forall env id tau,
-                   In (id, tau) env ->
-                     TPHasType env (TPId id) tau
+               TPIdHasTypeInEnv id env tau ->
+               TPHasType env (TPId id) tau
 | typerule_app: forall env exp1 exp2 tau tau',
-                    (TPHasType env exp1 (TPTypeFun tau tau')) ->
-                    (TPHasType env exp2 tau) ->
-                      (TPHasType env (TPApp exp1 exp2) tau')
+                (TPHasType env exp1 (TPTypeFun tau tau')) ->
+                (TPHasType env exp2 tau) ->
+                (TPHasType env (TPApp exp1 exp2) tau')
 | typerule_cond: forall env exp0 exp1 exp2 tau,
-                     (TPHasType env exp0 TPTypeBool) ->
-                     (TPHasType env exp1 tau) ->
-                     (TPHasType env exp2 tau) ->
-                       (TPHasType env (TPIf exp0 exp1 exp2) tau)
-| typerule_abstr: forall env env' exp id tau tau',
-                      env' = change_env id tau env ->
-                      (TPHasType env' exp tau') ->
-                      (TPHasType env (TPAbstr id exp) (TPTypeFun tau tau'))
-| typerule_rec: forall env env' exp id tau,
-                    env' = change_env id tau env ->
-                    (TPHasType env' exp tau) ->
-                    (TPHasType env (TPRec id exp) tau)
-| typerule_let: forall env env' exp1 exp2 id tau1 tau2,
-                    env' = change_env id tau1 env ->
-                    (TPHasType env exp1 tau1) ->
-                    (TPHasType env' exp2 tau2) ->
-                    (TPHasType env (TPLet id exp1 exp2) tau2).
+                 (TPHasType env exp0 TPTypeBool) ->
+                 (TPHasType env exp1 tau) ->
+                 (TPHasType env exp2 tau) ->
+                 (TPHasType env (TPIf exp0 exp1 exp2) tau)
+| typerule_abstr: forall env exp id tau tau' tau'',
+                  (TPHasType (TPChangeEnv env id tau) exp tau') ->
+                  tau'' = TPTypeFun tau tau' ->
+                  (TPHasType env (TPAbstr id exp) tau'')
+| typerule_rec: forall env exp id tau,
+                (TPHasType (TPChangeEnv env id tau) exp tau) ->
+                (TPHasType env (TPRec id exp) tau)
+| typerule_let: forall env exp1 exp2 id tau1 tau2,
+                (TPHasType env exp1 tau1) ->
+                (TPHasType (TPChangeEnv env id tau1) exp2 tau2) ->
+                (TPHasType env (TPLet id exp1 exp2) tau2).
 
-Lemma change_env_inversion: forall env env' id tau, env' = change_env id tau env -> TPHasType env' (TPId id) tau.
+Notation "Env |> exp ::: tau" := (TPHasType Env exp tau) (at level 10, no associativity).
+
+Definition TPWellTyped env exp := exists tau, env |> exp ::: tau.
+
+Lemma type_unique: forall exp env tau tau', env |> exp ::: tau -> env |> exp ::: tau' -> tau = tau'.
 Proof.
-  intros env env' id tau H.
-  induction env.
-    simpl in H. rewrite H. constructor. simpl. left. reflexivity.
-    destruct a as [id' tau']. constructor. rewrite H. simpl.
-    case_eq (ident_eq id id'); intros H'; simpl.
-      left. reflexivity.
-      right. apply change_env_consist.
+  intros exp env tau tau' Htau Htau'.
+  generalize dependent tau.
+  induction Htau'; intros tau''' Htau'''.
+    (**)
+    inversion_clear Htau'''.
+    rewrite H. rewrite H0. reflexivity.
+    (**)
+    inversion_clear Htau'''.
+    apply TypeOfIdUnique with (id:=id)(env:=env); assumption.
+    (**)
+    inversion_clear Htau'''.
+    specialize IHHtau'1 with (tau0:=(TPTypeFun tau0 tau''')).
+    assert (TPTypeFun tau0 tau''' = TPTypeFun tau tau'). apply IHHtau'1. assumption.
+    inversion H1. reflexivity.
+    (**)
+    inversion_clear Htau'''. apply IHHtau'2. assumption.
+    (**)
+    admit.
+    (**)
+    admit.
+    (**)
+    admit.
 Qed.
 
-Definition TPWellTyped env exp := exists tau, TPHasType env exp tau.
-
-Example test1: forall env, TPHasType env (TPApp TPPlus (TPInt 1)) TPTypeIntToInt.
+Lemma remove_unfree_ids: forall exp env id tau tau', TPIsNotFreeIn id exp -> (TPChangeEnv env id tau) |> exp ::: tau' -> env |> exp ::: tau'.
 Proof.
-  intros.
-  apply typerule_app with (tau:=TPTypeInt); apply typerule_const; simpl; reflexivity.
+  intros exp.
+  induction exp; intros env id' tau tau' Hnotfree Hexp.
+    (* TPConst *)
+    inversion_clear Hexp. rewrite H. constructor. reflexivity.
+    (* TPId *)
+    inversion_clear Hexp. constructor. inversion_clear Hnotfree.
+    apply TypeOfChangedEnvNeq with (id:=id')(tau:=tau); assumption.
+    (* TPApp *)
+    inversion_clear Hexp. inversion_clear Hnotfree. destruct H1 as [H1_1 H1_2].
+    apply typerule_app with (tau:=tau0).
+      apply IHexp1 with (id:=id')(tau:=tau); assumption.
+      apply IHexp2 with (id:=id')(tau:=tau); assumption.
+    (* TPAbstr *)
+    inversion_clear Hexp. inversion Hnotfree.
+      (* id = id' *)
+      clear H4 exp0 H1 id0. rewrite H0.
+      rewrite H3 in H. rewrite TypeOfDoubleChangeEnv in H.
+      apply typerule_abstr with (tau:=tau0)(tau':=tau'0).
+        assumption.
+        reflexivity.
+      (* id <> id' *)
+      clear H2 exp0 H1 id'0 H3 id0. rewrite H0.
+      apply typerule_abstr with (tau:=tau0)(tau':=tau'0).
+        apply IHexp with (id:=id')(tau:=tau).
+          assumption.
+          rewrite DoubleChangeSwitch.
+            assumption.
+            apply not_eq_sym. assumption.
+          reflexivity.
+    (* TPIf *)
+    inversion_clear Hexp. inversion_clear Hnotfree. destruct H2 as [H2_1 [H2_2 H2_3]].
+    constructor.
+      apply IHexp1 with (id:=id')(tau:=tau); assumption.
+      apply IHexp2 with (id:=id')(tau:=tau); assumption.
+      apply IHexp3 with (id:=id')(tau:=tau); assumption.
+    (* TPLet *)
+    inversion_clear Hexp. inversion_clear Hnotfree.
+    apply typerule_let with (tau1:=tau1).
+      apply IHexp1 with (id:=id')(tau:=tau); assumption.
+      destruct H1.
+        destruct H1 as [H1_1 H1_2].
+        apply IHexp2 with (id:=id')(tau:=tau).
+          assumption.
+          rewrite DoubleChangeSwitch.
+            assumption.
+            apply not_eq_sym. assumption.
+        rewrite <- TypeOfDoubleChangeEnv with (tau:=tau). rewrite <- H1 at 1. assumption.
+    (* TPRec *)
+    inversion_clear Hexp. inversion Hnotfree.
+      (* id = id' *)
+      clear H3 exp0 H0 id0. constructor. rewrite <- TypeOfDoubleChangeEnv with (tau:=tau).
+      rewrite <- H2 at 1. assumption.
+      (* id <> id' *)
+      clear H1 exp0 H0 id'0 H2 id0. constructor.
+      apply IHexp with (id:=id')(tau:=tau).
+        assumption.
+        rewrite DoubleChangeSwitch.
+            assumption.
+            apply not_eq_sym. assumption.
 Qed.
 
-Example test2: forall env, TPHasType env (TPApp (TPApp TPPlus (TPInt 1)) (TPInt 1)) TPTypeInt.
+Lemma add_unfree_ids: forall exp env id tau tau', TPIsNotFreeIn id exp -> env |> exp ::: tau' -> (TPChangeEnv env id tau) |> exp ::: tau'.
 Proof.
-  intros.
-  repeat (apply typerule_app with (tau:=TPTypeInt));
-    apply typerule_const; simpl; reflexivity.
+  intros exp.
+  induction exp; intros env id' tau tau' Hnotfree Hexp.
+    (* TPConst *)
+    inversion_clear Hexp. rewrite H. constructor. reflexivity.
+    (* TPId *)
+    inversion_clear Hexp. constructor. inversion_clear Hnotfree. constructor.
+      apply not_eq_sym. assumption.
+      assumption.
+    (* TPApp *)
+    inversion_clear Hexp. inversion_clear Hnotfree. destruct H1 as [H1_1 H1_2].
+    apply typerule_app with (tau:=tau0).
+      apply IHexp1; assumption.
+      apply IHexp2; assumption.
+    (* TPAbstr *)
+    inversion_clear Hexp. inversion Hnotfree.
+      (* id = id' *)
+      clear H4 exp0 H1 id0. apply typerule_abstr with (tau:=tau0)(tau':=tau'0).
+        rewrite TypeOfDoubleChangeEnv. assumption.
+        assumption. 
+      (* id <> id' *)
+      clear H2 exp0 H1 id'0 H3 id0. 
+      apply typerule_abstr with (tau:=tau0)(tau':=tau'0).
+        rewrite DoubleChangeSwitch.
+          apply IHexp; assumption.
+          assumption.
+        assumption.
+    (* TPIf *)
+    inversion_clear Hexp. inversion_clear Hnotfree. destruct H2 as [H2_1 [H2_2 H2_3]].
+    constructor.
+      apply IHexp1; assumption.
+      apply IHexp2; assumption.
+      apply IHexp3; assumption.
+    (* TPLet *)
+    inversion_clear Hexp. inversion_clear Hnotfree. apply typerule_let with (tau1:=tau1).
+      apply IHexp1; assumption.
+      destruct H1.
+        destruct H1 as [H1_1 H1_2]. rewrite DoubleChangeSwitch.
+          apply IHexp2; assumption.
+          assumption.
+        rewrite H1. rewrite TypeOfDoubleChangeEnv. assumption.
+    (* TPRec *)
+    inversion_clear Hexp. inversion Hnotfree.
+      (* id = id' *)
+      clear H3 exp0 H0 id0. constructor. rewrite TypeOfDoubleChangeEnv. assumption.
+      (* id <> id' *)
+      clear H1 exp0 H0 id'0 H2 id0. constructor. rewrite DoubleChangeSwitch.
+        apply IHexp; assumption.
+        assumption.
+Qed.
+
+Lemma substitution_and_typing : forall e e' exp id env tau tau',
+  env |> e ::: tau -> 
+  (TPChangeEnv env id tau) |> e' ::: tau' -> 
+  TPSubstitutesInto e' id e exp -> 
+  env |> exp ::: tau'.
+Proof.
+  intros e e' exp id env tau tau' He He' Hsubst.
+  generalize dependent He'.
+  generalize dependent He.
+  generalize dependent tau'.
+  generalize dependent tau.
+  generalize dependent env.
+  induction Hsubst; intros env tau tau' He He'.
+    (**)
+    inversion He'. clear H2 tau0 H0 env0 H c0. constructor. assumption.
+    (**)
+    inversion He'. clear H2 tau0 H id0 H0 env0.
+    inversion H1; clear H1.
+      (**)
+      rewrite H3 in H. clear H3 tau0 H0 id0. rewrite H2 in H. apply TPChangeEnv_prop1 in H. rewrite H. assumption.
+      (**)
+      clear H4 tau0 H2 id0. inversion_clear He'. 
+      assert (tau = tau'). apply TypeOfChangedEnvEq with (id:=id)(env:=env)(tau':=tau'). assumption.
+      rewrite <- H2. assumption.
+    (**)
+    inversion He'; clear H3 tau0 H0 id0 H1 env0.
+    constructor. apply TypeOfChangedEnvNeq with (id:=id)(tau:=tau); assumption.
+    (**)
+    inversion He'. clear H4 tau0 H1 exp2 H0 exp1 H exp0 H2 env0. constructor.
+      apply IHHsubst1 with (tau:=tau); assumption.
+      apply IHHsubst2 with (tau:=tau); assumption.
+      apply IHHsubst3 with (tau:=tau); assumption.
+    (**)
+    inversion He'. clear H3 tau'0 H0 exp2 H exp1 H1 env0.
+    apply typerule_app with (tau:=tau0).
+      apply IHHsubst1 with (tau:=tau); assumption.
+      apply IHHsubst2 with (tau:=tau); assumption.
+    (**)
+    inversion He'. clear H0 exp H id0 H1 env0.
+    assert ((TPChangeEnv (TPChangeEnv env id tau) id tau0) = (TPChangeEnv env id tau0)).
+      apply TypeOfDoubleChangeEnv with (tau:=tau).
+    rewrite H in H2. apply typerule_abstr with (tau:=tau0)(tau':=tau'0).
+      assumption.
+      assumption.
+    (**)
+    apply rename_function_prop in H0. destruct H0 as [H0_1 [H0_2 H0_3]].
+    inversion H0_3.
+      (* id' = id'' *)
+      clear H3 exp H0 id0. inversion He'. clear H5 tau'' H1 exp H0 id0 H3 env0.
+      apply typerule_abstr with (tau:=tau0)(tau':=tau'0).
+        apply IHHsubst2 with (tau:=tau).
+          apply add_unfree_ids.
+            rewrite H2 in H0_2. assumption.
+            assumption.
+          apply IHHsubst1 with (tau:=tau0).
+            constructor. rewrite H2. constructor.
+              apply not_eq_sym. assumption.
+              constructor. reflexivity.
+            rewrite DoubleChangeSwitch with (id:=id')(id':=id).
+              rewrite TypeOfDoubleChangeEnv. assumption.
+              apply not_eq_sym. assumption.
+            assumption.
+      (* id' <> id'' *)
+      clear H1 exp H0 id'0 H2 id0. inversion He'. clear H6 tau'' H1 exp H0 id0.
+      apply typerule_abstr with (tau:=tau0)(tau':=tau'0).
+        apply IHHsubst2 with (tau:=tau).
+          apply add_unfree_ids; assumption.
+          rewrite DoubleChangeSwitch.
+            apply IHHsubst1 with (tau:=tau0).
+              constructor. constructor. reflexivity.
+              rewrite DoubleChangeSwitch.
+                apply add_unfree_ids; assumption.
+                assumption.
+            apply not_eq_sym. assumption.
+          assumption.
+    (**)
+    inversion He'. clear H2 tau2 H3 exp2 H0 exp1 H id0.
+    apply typerule_let with (tau1:=tau1).
+      apply IHHsubst with (tau:=tau); assumption.
+      rewrite TypeOfDoubleChangeEnv in H5. assumption.
+    (**)
+    apply rename_function_prop in H0. destruct H0 as [H0_1 [H0_2 H0_3]].
+    inversion_clear H0_3. inversion_clear He'. destruct H0.
+      destruct H0 as [H0_1' H0_2'].
+      apply typerule_let with (tau1:=tau1).
+        apply IHHsubst1 with (tau:=tau); assumption.
+        apply IHHsubst3 with (tau:=tau).
+          apply add_unfree_ids; assumption.
+          rewrite DoubleChangeSwitch.
+            apply IHHsubst2 with (tau:=tau1).
+              constructor. constructor. reflexivity.
+              rewrite DoubleChangeSwitch.
+                apply add_unfree_ids; assumption.
+                assumption.
+            apply not_eq_sym. assumption.
+      rewrite H0. rewrite H0 in H0_2. rewrite H0 in Hsubst2.
+      rewrite H0 in IHHsubst2. rewrite H0 in H1. rewrite H0 in H0_1.
+      clear H0 id''.
+      apply typerule_let with (tau1:=tau1).
+        apply IHHsubst1 with (tau:=tau); assumption.
+        apply IHHsubst3 with (tau:=tau).
+          apply add_unfree_ids. assumption.
+          assumption.
+          rewrite DoubleChangeSwitch.
+            apply IHHsubst2 with (tau:=tau1).
+              constructor. constructor. reflexivity.
+              rewrite TypeOfDoubleChangeEnv. assumption.
+            apply not_eq_sym. assumption.
+    (**)
+    inversion_clear He'. rewrite TypeOfDoubleChangeEnv in H.
+    apply typerule_rec. assumption.
+    (**)
+    apply rename_function_prop in H0. destruct H0 as [H0_1 [H0_2 H0_3]].
+    inversion_clear He'. inversion H0_3.
+      (* id' = id'' *)
+      clear H4 exp H1 id0. apply typerule_rec. apply IHHsubst2 with (tau:=tau).
+        rewrite H3 in H0_2. apply add_unfree_ids; assumption.
+        rewrite DoubleChangeSwitch. apply IHHsubst1 with (tau:=tau').
+          rewrite H3. constructor. constructor. reflexivity.
+          rewrite TypeOfDoubleChangeEnv. assumption.
+      apply not_eq_sym. assumption.
+      (* id' <> id'' *)
+      clear H2 exp H1 id'0 H3 id0. apply typerule_rec. apply IHHsubst2 with (tau:=tau).
+        apply add_unfree_ids; assumption.
+        rewrite DoubleChangeSwitch. apply IHHsubst1 with (tau:=tau').
+          constructor. constructor. reflexivity.
+          rewrite DoubleChangeSwitch.
+            apply add_unfree_ids; assumption.
+            assumption.
+        apply not_eq_sym. assumption.
+Qed.
+
+Theorem preservation : forall env e e' tau, env |> e ::: tau -> TPMakesSmallstep e e' -> env |> e' ::: tau.
+Proof.
+  intros env e e' tau Hwelltyped Hsmallstep.
+  generalize dependent tau.
+  generalize dependent env.
+  induction Hsmallstep; intros env tau Hwelltyped.
+    (* Op *)
+    inversion_clear Hwelltyped.
+    inversion_clear H.
+    inversion_clear H1.
+    destruct op; simpl; simpl in H; inversion H; constructor; simpl; reflexivity.
+    (* Beta-V *)
+    inversion_clear Hwelltyped. inversion_clear H1. inversion H4.
+    rewrite <- H5 in H3.
+    apply substitution_and_typing with (e:=v)(e':=exp)(id:=id)(tau:=tau0).
+      assumption.
+      assumption.
+      assumption.
+    (* App-Left *)
+    inversion_clear Hwelltyped.
+    apply typerule_app with (tau:=tau0).
+      apply IHHsmallstep. assumption.
+      assumption.
+    (* App-Right *)
+    inversion_clear Hwelltyped.
+    apply typerule_app with (tau:=tau0).
+      assumption.
+      apply IHHsmallstep. assumption.
+    (* Cond-Eval *)
+    inversion_clear Hwelltyped.
+    constructor.
+      apply IHHsmallstep. assumption.
+      assumption.
+      assumption.
+    (* Cond-True *)
+    inversion_clear Hwelltyped. assumption.
+    (* Cond-False *)
+    inversion_clear Hwelltyped. assumption.
+    (* Let-Eval *)
+    inversion_clear Hwelltyped.
+    apply typerule_let with (tau1:=tau1).
+      apply IHHsmallstep.
+        assumption.
+      assumption.
+    (* Let-Exec *)
+    inversion_clear Hwelltyped.
+    apply substitution_and_typing with (e:=v)(e':=exp)(id:=id)(tau:=tau1).
+      assumption.
+      assumption.
+      assumption.
+    (* Unfold *)
+    inversion_clear Hwelltyped.
+    apply substitution_and_typing with (e:=(TPRec id exp))(e':=exp)(id:=id)(tau:=tau).
+      constructor. assumption.
+      assumption.
+      assumption.
+Qed.
+
+Definition TPClosed exp := forall id, TPIsNotFreeIn id exp.
+
+Lemma closed_app: forall exp1 exp2, TPClosed (TPApp exp1 exp2) -> (TPClosed exp1 /\ TPClosed exp2).
+Proof.
+  intros exp1 exp2 H.
+  unfold TPClosed in H. unfold TPClosed. split;
+    intros id; specialize H with (id:=id); inversion H; destruct H2; assumption.
+Qed.
+
+Lemma closed_if: forall exp1 exp2 exp3, TPClosed (TPIf exp1 exp2 exp3) -> (TPClosed exp1 /\ TPClosed exp2 /\ TPClosed exp3).
+Proof.
+  intros exp1 exp2 exp3 H.
+  unfold TPClosed in H. unfold TPClosed. split; try split;
+    intros id; specialize H with (id:=id); inversion H; destruct H2 as [H2_1 [H2_2 H2_3]]; assumption.
+Qed.
+
+Lemma bool_value: forall env exp, env |> exp ::: TPTypeBool -> TPIsValue exp -> exp = TPFalse \/ exp = TPTrue.
+Proof.
+  intros env exp Hwelltyped Hvalue.
+  induction Hvalue.
+    (**)
+    inversion Hwelltyped. destruct c; simpl in H1; try (contradict H1; now discriminate).
+      (**)
+      destruct b.
+        right; reflexivity.
+        left; reflexivity.
+      (**)
+      destruct op; simpl in H1; contradict H1; now discriminate.
+    (**)
+    inversion_clear Hwelltyped. contradict H0. discriminate.
+    (**)
+    inversion_clear Hwelltyped. inversion_clear H. destruct op; simpl in H1; contradict H1; discriminate.
+Qed.
+
+Lemma int_value: forall env exp, env |> exp ::: TPTypeInt -> TPIsValue exp -> exists n, exp = TPInt n.
+Proof.
+  intros env exp Hwelltyped Hvalue.
+  induction Hvalue.
+    (**)
+    inversion Hwelltyped. destruct c; simpl in H1; try (contradict H1; now discriminate).
+      (**)
+      exists n. reflexivity.
+      (**)
+      destruct op; simpl in H1; contradict H1; now discriminate.
+    (**)
+    inversion_clear Hwelltyped. contradict H0. discriminate.
+    (**)
+    inversion_clear Hwelltyped. inversion_clear H. destruct op; simpl in H1; contradict H1; discriminate.
+Qed.
+
+Lemma closed_rec: forall exp id, TPClosed (TPExpRec id exp) -> TPClosed exp \/ (exists id', TPIsFreeIn id' exp).
+Proof.
+  intros exp id H. unfold TPClosed in H. admit.
+Qed.
+
+Theorem progress: forall env tau e, env |> e ::: tau -> TPClosed e -> (exists e', TPMakesSmallstep e e') \/ TPIsValue e.
+Proof.
+  intros env tau e Hwelltyped Hclosed.
+  induction Hwelltyped.
+    (**)
+    right. constructor.
+    (**)
+    unfold TPClosed in Hclosed. specialize Hclosed with (id0:=id). inversion Hclosed. contradict H2. reflexivity.
+    (**)
+    left. apply closed_app in Hclosed. destruct Hclosed as [Hclosed1 Hclosed2].
+    destruct IHHwelltyped1 as [Hexp1 | Hexp1]. assumption.
+      (* exp1 makes smallstep *)
+      destruct Hexp1 as [exp1' Hexp1]. exists (TPApp exp1' exp2).
+      constructor. assumption.
+      (* exp1 is value *)
+      destruct IHHwelltyped2 as [Hexp2 | Hexp2]. assumption.
+        (* exp2 makes smallstep *)
+        destruct Hexp2 as [exp2' Hexp2]. exists (TPApp exp1 exp2').
+        constructor; assumption.
+        (* exp2 is value *)
+        inversion Hexp1.
+          rewrite <- H in Hwelltyped1. inversion Hwelltyped1. destruct c; try (simpl in H2; contradict H2; discriminate).
+          (* exp2 is operator *)
+          admit.
+          (* exp2 is abstraction *)
+          rewrite <- H in Hwelltyped1. inversion Hwelltyped1.
+            admit.
+            admit.
+    (**)
+    left. apply closed_if in Hclosed. destruct Hclosed as [Hclosed0 [Hclosed1 Hclosed2]].
+    destruct IHHwelltyped1 as [Hexp0 | Hexp0]. assumption.
+      (* exp0 makes smallstep *)
+      destruct Hexp0 as [exp0' Hexp0]. exists (TPIf exp0' exp1 exp2).
+      constructor. assumption.
+      (* exp0 is value *)
+      assert (exp0 = TPFalse \/ exp0 = TPTrue).
+        apply bool_value with (env:=env); assumption.
+      destruct H.
+        (* exp0 = TPFalse *)
+        exists exp2. rewrite H. constructor.
+        (* exp0 = TPTrue *)
+        exists exp1. rewrite H. constructor.
+    (**)
+    right. constructor.
+    (**)
+    assert (TPIsNotFreeIn id (TPRec id exp)).
+      apply Hclosed.
+    inversion H.
+      left. exists exp. constructor.
+      admit.
+    admit.
+    (**)
+    left. admit.
 Qed.
 
 End TPTyping.
