TPSemanticFreeVariables.v
@@ -1,0 +1,107 @@
+Module TPSemanticFreeVariables.
+
+Load TPSyntaxExpressions.
+Export TPSyntaxExpressions.
+
+Load TPSyntaxIdentifiers.
+Export TPSyntaxIdentifiers.
+
+Inductive TPIsFreeIn: TPIdentifier -> TPExp -> Prop :=
+| free_id: forall id, TPIsFreeIn id (TPExpId id)
+| free_app: forall id exp1 exp2, (TPIsFreeIn id exp1 \/ TPIsFreeIn id exp2) -> TPIsFreeIn id (TPExpApp exp1 exp2)
+| free_if: forall id exp1 exp2 exp3, (TPIsFreeIn id exp1 \/ TPIsFreeIn id exp2 \/ TPIsFreeIn id exp3) -> TPIsFreeIn id (TPExpIf exp1 exp2 exp3)
+| free_abstr: forall id id' exp, id <> id' ->  TPIsFreeIn id exp -> TPIsFreeIn id (TPExpAbstr id' exp)
+| free_let: forall id id' exp' exp, (id <> id' /\ TPIsFreeIn id exp) \/ TPIsFreeIn id exp' -> TPIsFreeIn id (TPExpLet id' exp' exp)
+| free_rec: forall id id' exp, id <> id' -> TPIsFreeIn id exp -> TPIsFreeIn id (TPExpRec id' exp).
+
+Inductive TPIsNotFreeIn: TPIdentifier -> TPExp -> Prop :=
+| notfree_const: forall id c, TPIsNotFreeIn id (TPExpConst c)
+| notfree_id: forall id id', id <> id' -> TPIsNotFreeIn id (TPExpId id')
+| notfree_app: forall id exp1 exp2, (TPIsNotFreeIn id exp1 /\ TPIsNotFreeIn id exp2) -> TPIsNotFreeIn id (TPExpApp exp1 exp2)
+| notfree_if: forall id exp1 exp2 exp3, (TPIsNotFreeIn id exp1 /\ TPIsNotFreeIn id exp2 /\ TPIsNotFreeIn id exp3) -> TPIsNotFreeIn id (TPExpIf exp1 exp2 exp3)
+| notfree_abstr_eq: forall id exp, TPIsNotFreeIn id (TPExpAbstr id exp)
+| notfree_abstr_neq: forall id id' exp, id <> id' -> TPIsNotFreeIn id exp -> TPIsNotFreeIn id (TPExpAbstr id' exp)
+| notfree_let: forall id id' exp' exp, ((TPIsNotFreeIn id exp /\ id <> id') \/ id = id') -> TPIsNotFreeIn id exp' -> TPIsNotFreeIn id (TPExpLet id' exp' exp)
+| notfree_rec_eq: forall id exp, TPIsNotFreeIn id (TPExpRec id exp)
+| notfree_rec_neq: forall id id' exp, id <> id' -> TPIsNotFreeIn id exp -> TPIsNotFreeIn id (TPExpRec id' exp).
+
+Lemma TPIsNotFreeIn_consist: forall exp id, ~ TPIsFreeIn id exp <-> TPIsNotFreeIn id exp.
+Proof.
+  intros exp id. split; intros H.
+  (* => *)
+  generalize dependent id.
+  induction exp; intros id' H.
+    (**)
+    constructor.
+    (**)
+    constructor. compute in H. intros H'. apply H. rewrite H'. constructor.
+    (**)
+    constructor. compute in H. split.
+      apply IHexp1. intros H'. apply H. constructor. left. assumption. 
+      apply IHexp2. intros H'. apply H. constructor. right. assumption.
+    (**)
+    case_eq (ident_eq id' id); intros Hid.
+      apply ident_eq_consist in Hid. rewrite Hid. constructor.
+      apply ident_eq_consist_conv in Hid. constructor.
+        assumption. 
+        compute in H. apply IHexp. intros H'. apply H. constructor.
+          assumption.
+          assumption.
+    (**)
+    constructor. compute in H. split.
+      apply IHexp1. intros H'. apply H. constructor. left. assumption.
+      split.
+        apply IHexp2. intros H'. apply H. constructor. right. left. assumption.
+        apply IHexp3. intros H'. apply H. constructor. right. right. assumption.
+    (**)
+    compute in H. constructor. case_eq (ident_eq id' id); intros Hid.
+      apply ident_eq_consist in Hid. right. assumption.
+      apply ident_eq_consist_conv in Hid. left. split. 
+        apply IHexp2. intros H'. apply H. constructor. left. split; assumption.
+        assumption.
+    (**)
+    compute in H. case_eq (ident_eq id' id); intros Hid.
+      apply ident_eq_consist in Hid. rewrite Hid. apply IHexp1. intros H'. apply H. constructor. right. rewrite Hid. assumption.
+      apply ident_eq_consist_conv in Hid. apply IHexp1. intros H'. apply H. constructor. right. assumption. 
+    (**)
+    compute in H. case_eq (ident_eq id' id); intros Hid. 
+      apply ident_eq_consist in Hid. rewrite Hid. constructor.
+      apply ident_eq_consist_conv in Hid. constructor.
+        assumption.
+        apply IHexp. intros H'. apply H. constructor; assumption.
+  (* <= *)
+  generalize dependent id. induction exp; intros id' H H'.
+    (**)
+    inversion_clear H. inversion_clear H'.
+    (**)
+    inversion_clear H. inversion H'. contradiction.
+    (**)
+    inversion_clear H. inversion_clear H'. destruct H0. destruct H.
+      contradict H. apply IHexp1. assumption.
+      contradict H. apply IHexp2. assumption.
+    (**)
+    inversion H.
+      inversion_clear H'. contradict H1. assumption.
+      inversion_clear H'. specialize IHexp with (id:=id'). destruct IHexp; assumption.
+    (**)
+    inversion_clear H. inversion_clear H'. destruct H0. destruct H1. destruct H as [H | [H | H]].
+      contradict H. apply IHexp1. assumption.
+      contradict H. apply IHexp2. assumption.
+      contradict H. apply IHexp3. assumption.
+    (**)
+    inversion_clear H'. destruct H0 as [[H0 H1] | H0].
+      inversion_clear H. destruct H2 as [H2 | H2].
+        specialize IHexp2 with (id:=id'). destruct H2 as [H2_1 H2_2]. destruct IHexp2; assumption.
+        contradict H0. assumption.
+      inversion_clear H. destruct H1 as [H1 | H1];
+        specialize IHexp1 with (id:=id'); destruct IHexp1; assumption.
+    (**)
+    inversion H.
+      inversion_clear H'. contradict H1. assumption.
+      inversion_clear H'. specialize IHexp with (id:=id'). destruct IHexp. assumption. assumption.
+Qed.
+
+Lemma TPIsFreeIn_consist: forall exp id, ~ TPIsNotFreeIn id exp <-> TPIsFreeIn id exp.
+Admitted.
+
+End TPSemanticFreeVariables.
