TPSyntaxConstants.v
@@ -1,0 +1,65 @@
+Module TPSyntaxConstants.
+
+Require Export ZArith.
+
+Load TPSyntaxOperators.
+Export TPSyntaxOperators.
+
+Inductive TPConstant :=
+ | TPConstantUnit
+ | TPConstantBool (b : bool)
+ | TPConstantInt (n : Z)
+ | TPConstantOp (op : TPOperator)
+ | TPConstantExn
+ | TPConstantHang.
+
+(* Boolean version of constant equality *)
+Fixpoint TPConstant_eq c1 c2 :=
+  match c1, c2 with
+    | TPConstantUnit, TPConstantUnit => true
+    | TPConstantBool b1, TPConstantBool b2 => bool_eq b1 b2
+    | TPConstantInt n1, TPConstantInt n2 => Zeq_bool n1 n2
+    | TPConstantOp op1, TPConstantOp op2 => TPOperator_eq op1 op2
+    | TPConstantExn, TPConstantExn => true
+    | TPConstantHang, TPConstantHang => true
+    | _, _ => false
+  end.
+
+(* Consistency lemma *)
+Lemma TPConstant_eq_consist: forall c1 c2: TPConstant, TPConstant_eq c1 c2 = true <-> c1 = c2.
+Proof.
+  intros c1 c2.
+  split; intros H.
+    (* => *)
+    destruct c1; destruct c2; simpl in H; try (discriminate || reflexivity).
+    apply bool_eq_ok in H; rewrite H; reflexivity.
+    apply Zeq_bool_eq in H; rewrite H; reflexivity.
+    apply TPOperator_eq_consist in H; rewrite H; reflexivity.
+    (* <= *)
+    destruct c1; destruct c2; simpl in H; simpl; try discriminate; try reflexivity.
+    inversion H. destruct b0; reflexivity.
+    inversion H. apply Zeq_is_eq_bool. reflexivity.
+    inversion H. apply TPOperator_eq_consist. reflexivity.
+Qed.
+
+Lemma TPConstant_eq_reflex: forall c: TPConstant, TPConstant_eq c c = true.
+Proof.
+  intros c.
+  induction c; simpl.
+    (* Case TPunit*)
+    now reflexivity.
+    (* Case TPbool*)
+    destruct b; simpl; now reflexivity.
+    (* Case TPint*)
+    induction n. compute. reflexivity.
+    induction p; auto.
+    induction p; auto.
+    (* Case TPop*)
+    now apply TPOperator_eq_reflex.
+    (* Case TPexn*)
+    now reflexivity.
+    (* Case TPhang*)
+    now reflexivity.
+Qed.
+
+End TPSyntaxConstants.
