TPSyntaxExpressions.v
@@ -1,0 +1,192 @@
+Module TPSyntaxExpressions.
+
+Load TPSyntaxConstants.
+Export TPSyntaxConstants.
+
+Load TPSyntaxIdentifiers.
+Import TPSyntaxIdentifiers.
+
+Inductive TPExp :=
+ | TPExpConst (c : TPConstant)
+ | TPExpId (id : TPIdentifier)
+ | TPExpApp (a b : TPExp)
+ | TPExpAbstr (id : TPIdentifier) (exp : TPExp)
+ | TPExpIf (exp1 exp2 exp3 : TPExp)
+ | TPExpLet (id : string * nat) (exp1 exp2 : TPExp)
+ | TPExpRec (id : string * nat) (exp : TPExp).
+
+(* Shorthands *)
+Definition TPOp op := (TPExpConst (TPConstantOp op)).
+
+Definition TPUnit := (TPExpConst TPConstantUnit).
+Definition TPBool b := (TPExpConst (TPConstantBool b)).
+Definition TPFalse := (TPExpConst (TPConstantBool false)).
+Definition TPTrue := (TPExpConst (TPConstantBool true)).
+Definition TPInt n := (TPExpConst (TPConstantInt n)).
+
+Definition TPPlus := (TPExpConst (TPConstantOp TPOperatorPlus)).
+Definition TPMinus := (TPExpConst (TPConstantOp TPOperatorMinus)).
+Definition TPMult := (TPExpConst (TPConstantOp TPOperatorMult)).
+Definition TPDiv := (TPExpConst (TPConstantOp TPOperatorDiv)).
+Definition TPMod := (TPExpConst (TPConstantOp TPOperatorMod)).
+Definition TPLess := (TPExpConst (TPConstantOp TPOperatorLess)).
+Definition TPLessEq := (TPExpConst (TPConstantOp TPOperatorLessEq)).
+Definition TPGreater := (TPExpConst (TPConstantOp TPOperatorGreater)).
+Definition TPGreaterEq := (TPExpConst (TPConstantOp TPOperatorGreaterEq)).
+Definition TPEq := (TPExpConst (TPConstantOp TPOperatorEq)).
+Definition TPNeq := (TPExpConst (TPConstantOp TPOperatorNeq)).
+
+Definition TPExn := (TPExpConst TPConstantExn).
+Definition TPHang := (TPExpConst TPConstantHang).
+
+Definition TPConst c := TPExpConst c.
+Definition TPId id := TPExpId id.
+Definition TPApp a b := TPExpApp a b.
+Definition TPAbstr id exp := TPExpAbstr id exp.
+Definition TPIf exp1 exp2 exp3 := TPExpIf exp1 exp2 exp3.
+Definition TPLet id exp1 exp2 := TPExpLet id exp1 exp2.
+Definition TPRec id exp := TPExpRec id exp.
+
+(* Boolean version of expression equality *)
+Fixpoint TPExp_eq exp1 exp2 :=
+  match exp1, exp2 with
+    | TPExpConst c1, TPExpConst c2 => TPConstant_eq c1 c2
+    | TPExpId (id1, n1), TPExpId (id2, n2) => andb (string_eq id1 id2) (beq_nat n1 n2)
+    | TPExpApp exp11 exp12, TPExpApp exp21 exp22 =>
+      andb (TPExp_eq exp11 exp21) (TPExp_eq exp12 exp22)
+    | TPExpAbstr (id1, n1) exp1, TPExpAbstr (id2, n2) exp2 =>
+      andb (string_eq id1 id2) (andb (beq_nat n1 n2) (TPExp_eq exp1 exp2))
+    | TPExpIf e11 e12 e13, TPExpIf e21 e22 e23 =>
+      andb (TPExp_eq e11 e21) (andb (TPExp_eq e12 e22) (TPExp_eq e13 e23))
+    | TPExpLet (id1, n1) e11 e12, TPExpLet (id2, n2) e21 e22 =>
+      andb (string_eq id1 id2) (andb (beq_nat n1 n2) (andb (TPExp_eq e11 e21) (TPExp_eq e12 e22)))
+    | TPExpRec (id1, n1) e1, TPExpRec (id2, n2) e2 =>
+      andb (string_eq id1 id2) (andb (beq_nat n1 n2) (TPExp_eq e1 e2))
+    | _, _ => false
+  end.
+
+(* Consistency lemma *)
+Lemma TPExp_eq_consist: forall exp1 exp2: TPExp, (TPExp_eq exp1 exp2) = true <-> exp1 = exp2.
+Proof.
+  intros exp1 exp2.
+  split; intros H.
+    (* => *)
+    generalize dependent exp2.
+    (* The following creates all possible cases of exp1 and exp2 and immediately
+       solves all cases where the constructors of exp1 and exp2 are different. *)
+    induction exp1; destruct exp2; intros H; try discriminate; simpl in H;
+      try (induction id; now intuition); try induction id; try induction id0.
+    (* Case: TPExpConst *)
+    apply TPConstant_eq_consist in H; rewrite H; now reflexivity.
+    (* Case: TPExpId *)
+    apply andb_prop in H; destruct H; apply string_eq_consist in H.
+    symmetry in H0; apply beq_nat_eq in H0; rewrite H; rewrite H0; now reflexivity.
+    (* Case: TPExpApp *)
+    apply andb_prop in H; destruct H as [H H'].
+    rewrite IHexp1_1 with (exp2:=exp2_1).
+    rewrite IHexp1_2 with (exp2:=exp2_2).
+    now reflexivity. now exact H'. now exact H.
+    (* Case: TPExpAbstr *)
+    apply andb_prop in H. destruct H as [H H'].
+    apply string_eq_consist in H; rewrite H.
+    rewrite IHexp1 with (exp2:=exp2).
+    apply andb_prop in H'.
+    destruct H'; symmetry in H0; apply beq_nat_eq in H0; rewrite H0; now reflexivity.
+    apply andb_prop in H'; destruct H' as [H0 H1]; now exact H1.
+    (* Case: TPExpIf *)
+    apply andb_prop in H; destruct H as [H H'];
+    apply andb_prop in H'; destruct H' as [H' H''].
+    rewrite IHexp1_1 with (exp2:=exp2_1).
+    rewrite IHexp1_2 with (exp2:=exp2_2).
+    rewrite IHexp1_3 with (exp2:=exp2_3).
+    now reflexivity. now exact H''. now exact H'. now exact H.
+    (* Case: TPExpLet *)
+    apply andb_prop in H; destruct H as [H H'];
+    apply andb_prop in H'; destruct H' as [H' H''].
+    apply string_eq_consist in H; rewrite H.
+    apply andb_prop in H''; destruct H''.
+    rewrite IHexp1_1 with (exp2:=exp2_1).
+    rewrite IHexp1_2 with (exp2:=exp2_2).
+    symmetry in H'; apply beq_nat_eq in H'; rewrite H'; now reflexivity.
+    now exact H1. now exact H0.
+    (* Case: TPExpRec *)
+    apply andb_prop in H; destruct H as [H H'].
+    apply string_eq_consist in H; rewrite H.
+    rewrite IHexp1 with (exp2:=exp2); apply andb_prop in H'; destruct H'.
+    symmetry in H0; apply beq_nat_eq in H0; rewrite H0; now reflexivity.
+    now exact H1.
+    (* <= *)
+    rewrite H; clear H; clear exp1; induction exp2; simpl; try induction id.
+    (* Case TPExpConst *)
+    now apply TPConstant_eq_reflex.
+    (* Case TPExpId *)
+    apply andb_true_intro; split.
+    now apply string_eq_reflex.
+    symmetry; now apply beq_nat_refl.
+    (* Case TPExpApp *)
+    apply andb_true_intro; split; now assumption.
+    (* Case TPExpAbstr *)
+    apply andb_true_intro; split.
+    now apply string_eq_reflex.
+    apply andb_true_intro; split.
+    symmetry; now apply beq_nat_refl.
+    now exact IHexp2.
+    (* Case TPExpIf *)
+    rewrite IHexp2_1; rewrite IHexp2_2; simpl; now exact IHexp2_3.
+    (* Case TPExpLet *)
+    rewrite string_eq_reflex; rewrite IHexp2_1; rewrite IHexp2_2; 
+    simpl; apply andb_true_intro; split.
+    symmetry; now apply beq_nat_refl.
+    now reflexivity.
+    (* Case TPExpRec *)
+    rewrite string_eq_reflex; rewrite IHexp2; simpl; apply andb_true_intro; split; symmetry.
+    now apply beq_nat_refl. now reflexivity.
+Qed.
+
+Inductive TPIsValue: TPExp -> Prop :=
+| TPConstIsValue: forall c, TPIsValue (TPExpConst c)
+| TPAbstrIsValue: forall id exp, TPIsValue (TPAbstr id exp)
+| TPAppIsValue: forall op exp, TPIsValue exp -> TPIsValue (TPApp (TPOp op) exp).
+
+Fixpoint TPIsValue_bool (exp : TPExp) : bool :=
+  match exp with
+    | TPExpConst _ => true
+    | TPExpAbstr _ _ => true
+    | TPExpApp (TPExpConst (TPConstantOp _)) exp => TPIsValue_bool exp
+    | _ => false
+  end.
+
+Lemma TPIsValue_consist: forall exp, TPIsValue_bool exp = true <-> TPIsValue exp.
+Proof.
+  intros exp. split; intros H.
+  (* => *)
+    induction exp; try ((contradict H; discriminate) || constructor).
+    (* Case exp: TPExpApp *)
+    destruct exp1; simpl in H; try (contradict H; discriminate).
+      destruct c; try (contradict H; discriminate).
+      constructor. apply IHexp2. exact H.
+  (* <= *)
+    induction exp; inversion H; simpl; try reflexivity.
+    (* Case: TPOp *)
+    apply IHexp2. exact H1.
+Qed.
+
+Lemma TPIsValue_cases: forall exp, TPIsValue exp <-> (exists c, exp = TPConst c) \/ (exists id, exists exp', exp = TPAbstr id exp') \/ (exists op, exists exp', (exp = TPApp (TPOp op) exp' /\ TPIsValue exp')).
+Proof.
+  intros exp. split; intros H.
+  (* => *)
+  inversion H.
+    left. exists c. reflexivity.
+    right. left. exists id. exists exp0. reflexivity.
+    right. right. exists op. exists exp0. split.
+      reflexivity.
+      exact H0.
+    (* <= *)
+    destruct H as [[c H] | [[id [exp' H]] | [op [exp' [H H']]]]].
+      rewrite H. constructor.
+      rewrite H. constructor.
+      rewrite H. constructor. exact H'.
+Qed.
+
+End TPSyntaxExpressions.
+
