TPSyntaxIdentifiers.v
@@ -1,0 +1,147 @@
+Module TPSyntaxIdentifiers.
+
+Require Export String.
+Require Import Ascii.
+Require Import Arith.
+
+(* Very ugly boolean version of ascii equality *)
+Definition ascii_eq a1 a2 := match a1, a2 with
+| Ascii b1 b2 b3 b4 b5 b6 b7 b8, Ascii b1' b2' b3' b4' b5' b6' b7' b8'
+  => (bool_eq b1 b1' && bool_eq b2 b2' && bool_eq b3 b3' &&
+      bool_eq b4 b4' && bool_eq b5 b5' && bool_eq b6 b6' &&
+      bool_eq b7 b7' && bool_eq b8 b8')%bool
+end.
+
+(* Consistency Lemma *)
+Lemma ascii_eq_consist: forall a1 a2: ascii, ascii_eq a1 a2 = true <-> a1 = a2.
+Proof.
+  intros a1 a2.
+  split; intros H.
+  (* => *)
+    destruct a1 as [b1 b2 b3 b4 b5 b6 b7 b8].
+    destruct a2 as [b1' b2' b3' b4' b5' b6' b7' b8'].
+    simpl in H.
+    repeat (apply andb_prop in H; destruct H).
+    apply bool_eq_ok in H; rewrite H.
+    apply bool_eq_ok in H0; rewrite H0.
+    apply bool_eq_ok in H1; rewrite H1.
+    apply bool_eq_ok in H2; rewrite H2.
+    apply bool_eq_ok in H3; rewrite H3.
+    apply bool_eq_ok in H4; rewrite H4.
+    apply bool_eq_ok in H5; rewrite H5.
+    apply bool_eq_ok in H6; rewrite H6.
+    reflexivity.
+  (* <= *)
+    rewrite <- H. destruct a1 as [b1 b2 b3 b4 b5 b6 b7 b8]; simpl.
+    destruct b1; simpl;
+    destruct b2; simpl;
+    destruct b3; simpl;
+    destruct b4; simpl;
+    destruct b5; simpl;
+    destruct b6; simpl;
+    destruct b7; simpl;
+    destruct b8; simpl; reflexivity.
+Qed.
+
+Lemma ascii_eq_reflex: forall a: ascii, ascii_eq a a = true.
+Proof.
+  intros. destruct a as [b1 b2 b3 b4 b5 b6 b7 b8].
+  destruct b1; simpl;
+  destruct b2; simpl;
+  destruct b3; simpl;
+  destruct b4; simpl;
+  destruct b5; simpl;
+  destruct b6; simpl;
+  destruct b7; simpl;
+  destruct b8; simpl; reflexivity.
+Qed.
+
+(* Boolean version of string equality *)
+Fixpoint string_eq s1 s2 := match s1, s2 with
+| EmptyString, EmptyString => true
+| String a1 s1', String a2 s2' => if ascii_eq a1 a2 then string_eq s1' s2' else false
+| _, _ => false
+end.
+
+(* Consistency Lemma *)
+Lemma string_eq_consist: forall s1 s2: string, string_eq s1 s2 = true <-> s1 = s2.
+Proof.
+  split; intros H.
+    generalize dependent s2.
+    (* => *)
+    induction s1; destruct s2; intros H; simpl in H.
+      (* Base case *)
+      now reflexivity.
+      (* Base case *)
+      contradict H. now discriminate.
+      (* Step *)
+      contradict H. now discriminate.
+      (* Step *)
+        case_eq (ascii_eq a a0); intros; rewrite H0 in H.
+        (* Case: true *)
+        apply ascii_eq_consist in H0. rewrite H0.
+        specialize IHs1 with (s2:=s2). rewrite IHs1.
+        reflexivity. exact H.
+        (* Case: false *)
+        contradict H. discriminate.
+   (* <= *)
+    rewrite H. clear H. clear s1.
+    induction s2; simpl.
+      (* Base case *)
+      reflexivity.
+      (* Step *)
+      rewrite ascii_eq_reflex. exact IHs2.
+Qed.
+
+Lemma string_eq_reflex: forall s: string, string_eq s s = true.
+Proof.
+  intros s.
+  induction s; simpl.
+    (* Base case *)
+    now reflexivity.
+    (* Step *)
+    rewrite ascii_eq_reflex. now exact IHs.
+Qed.
+
+(* Boolean version of string inequality *)
+Definition string_neq s1 s2 := negb (string_eq s1 s2).
+
+Definition TPIdentifier: Set := (string * nat)%type.
+
+(* Boolean version of identifier inequality *)
+Definition ident_eq i1 i2 :=
+  match i1, i2 with
+    | (id1, num1), (id2, num2) => andb (string_eq id1 id2) (beq_nat num1 num2)
+  end.
+
+Lemma ident_eq_reflex: forall id, ident_eq id id = true.
+Proof.
+  induction id.
+  simpl.
+  apply andb_true_intro.
+  split.
+  now apply string_eq_reflex.
+  apply beq_nat_true_iff.
+  reflexivity.
+Qed.
+
+(* Consistency Lemma *)
+Lemma ident_eq_consist: forall id1 id2, ident_eq id1 id2 = true <-> id1 = id2.
+Proof.
+  induction id1; induction id2; simpl.
+  split; intro H.
+  (* => *)
+    apply andb_prop in H.
+    destruct H as [H1 H2].
+    apply string_eq_consist in H1.
+    symmetry in H2; apply beq_nat_eq in H2.
+    rewrite H1; rewrite H2; now reflexivity.
+  (* <= *)
+    apply andb_true_intro.
+    split; [apply string_eq_consist | apply beq_nat_true_iff]; inversion H; reflexivity.
+Qed.
+
+Lemma ident_eq_consist_conv: forall id id', ident_eq id id' = false <-> id <> id'.
+Admitted.
+
+End TPSyntaxIdentifiers.
