TPSyntaxOperators.v
@@ -1,0 +1,50 @@
+Module TPSyntaxOperators.
+
+Inductive TPOperator :=
+ | TPOperatorPlus
+ | TPOperatorMinus
+ | TPOperatorMult
+ | TPOperatorDiv
+ | TPOperatorMod
+ | TPOperatorLess
+ | TPOperatorLessEq
+ | TPOperatorGreater
+ | TPOperatorGreaterEq
+ | TPOperatorEq
+ | TPOperatorNeq.
+
+(* Boolean version of operator equality *)
+Definition TPOperator_eq op1 op2 :=
+  match op1, op2 with
+    | TPOperatorPlus, TPOperatorPlus => true
+    | TPOperatorMinus, TPOperatorMinus => true
+    | TPOperatorMult, TPOperatorMult => true
+    | TPOperatorDiv, TPOperatorDiv => true
+    | TPOperatorMod, TPOperatorMod => true
+    | TPOperatorLess, TPOperatorLess => true
+    | TPOperatorLessEq, TPOperatorLessEq => true
+    | TPOperatorGreater, TPOperatorGreater => true
+    | TPOperatorGreaterEq, TPOperatorGreaterEq => true
+    | TPOperatorEq, TPOperatorEq => true
+    | TPOperatorNeq, TPOperatorNeq => true
+    | _, _ => false
+  end.
+
+(* Consistency lemma *)
+Lemma TPOperator_eq_consist: forall op1 op2, TPOperator_eq op1 op2 = true <-> op1 = op2.
+Proof.
+  intros op1 op2.
+  split; intros H.
+    (* => *)
+    destruct op1; destruct op2; (discriminate || reflexivity).
+    (* <= *)
+    destruct op1; destruct op2; simpl; solve [discriminate | reflexivity].
+Qed.
+
+Lemma TPOperator_eq_reflex: forall op, TPOperator_eq op op = true.
+Proof.
+  intros op.
+  destruct op; simpl; reflexivity.
+Qed.
+
+End TPSyntaxOperators.
